More work on Hoare and the first half (or so) of SmallStep

SoftwareFoundations/ProgrammingLanguageFoundations/HoareAsLogic.lean
@@ -2,7 +2,14 @@
 # Hoare Logic as a Logic
 -/
 
+import SoftwareFoundations.LogicalFoundations.Maps
+import SoftwareFoundations.LogicalFoundations.Imp
+import SoftwareFoundations.ProgrammingLanguageFoundations.Hoare
+
 namespace SoftwareFoundations.ProgrammingLanguageFoundations.Hoare
+  open SoftwareFoundations.LogicalFoundations.Maps
+  open SoftwareFoundations.LogicalFoundations.Imp
+
   /-
   ## Hoare Logic and Model Theory
   -/
@@ -15,9 +22,42 @@ namespace SoftwareFoundations.ProgrammingLanguageFoundations.Hoare
   ## Derivability
   -/
 
+  inductive HoareLogic: Assertion → Command → Assertion → Type :=
+    | skip {P: Assertion}: HoareLogic P .skip P
+    | assign {Q: Assertion} {id: String} {e: Arith}: HoareLogic [Assert| ‹Q› [ ‹id› ↦ ‹e› ]] [Imp| ‹id› := ‹e› ] Q
+    | seq {P Q R: Assertion} {c₁ c₂: Command} (h₁: HoareLogic Q c₂ R) (h₂: HoareLogic P c₁ Q): HoareLogic P [Imp| ‹c₁›; ‹c₂› ] R
+    | if {P Q: Assertion} {c: Logic} {t f: Command} (h₁: HoareLogic _ t Q) (h₂: HoareLogic _ f Q): HoareLogic P [Imp| ite (‹c›) { ‹t› } else { ‹f› }] Q
+    | while {P: Assertion} {c: Logic} {b: Command} (h₁: HoareLogic _ b P): HoareLogic P [Imp| while (‹c›) { ‹b› }] _
+    | consequence {P₁ P₂ Q₁ Q₂: Assertion} {c: Command} (h₁: HoareLogic P₂ c Q₂) (h₂: (s: State) → P₁ s → P₂ s) (h₃: (s: State) → Q₂ s → Q₁ s): HoareLogic P₁ c Q₁
+
+  namespace Term
+    example (P₁ P₂ Q: Assertion) (c: Command) (h₁: HoareLogic P₂ c Q) (h₂: (s: State) → P₁ s → P₂ s): HoareLogic P₁ c Q := sorry
+    example (P Q₁ Q₂: Assertion) (c: Command) (h₁: HoareLogic P c Q₂) (h₂: (s: State) → Q₂ s → Q₁ s): HoareLogic P c Q₁ := sorry
+
+    example: [Hoare| ⦃(X = 3) [X ↦ X + 2] [X ↦ X + 1]⦄ X := X + 1; X := X + 2 ⦃(X = 3)⦄] := sorry
+
+    theorem HoareLogic.true_post {P: Assertion} {c: Command}: HoareLogic P c True := sorry
+    theorem HoareLogic.false_pre {Q: Assertion} {c: Command}: HoareLogic False c Q := sorry
+  end Term
+
   /-
   ## Soundness and Completeness
   -/
+
+  def _root_.SoftwareFoundations.ProgrammingLanguageFoundations.Hoare.Assertion.weakestPrecondition (Q: Assertion) (c: Command)
+    | s₁, s₂ => (s₁ =[c]=> s₂) → Q s₂
+
+  namespace Term
+    theorem HoareLogic.sound {P Q: Assertion} {c: Command} (h: HoareLogic P c Q): HoareTriple P c Q := sorry
+
+    theorem Assertion.weakestPrecondition.is_precondition {Q: Assertion} {c: Command}: [Hoare| ⦃ ‹Q.weakestPrecondition c› ⦄ ‹c› ⦃ ‹Q› ⦄] := sorry
+    theorem Assertion.weakestPrecondition.is_weakest {P Q: Assertion} {c: Command} (h: [Hoare| ⦃ ‹P› ⦄ ‹c› ⦃ ‹Q› ⦄]): [Assert| ‹P› → ‹Q.weakestPrecondition c›] := sorry
+
+    theorem Assertion.weakestPrecondition.seq {P Q: Assertion} {c₁ c₂: Command} (h₁: HoareLogic P c₁ (Q.weakestPrecondition c₂)) (h₂: HoareLogic (Q.weakestPrecondition c₂) c₂ Q): HoareLogic P [Imp| ‹c₁›; ‹c₂›] Q := sorry
+    theorem Assertion.weakestPrecondition.invariant {Q: Assertion} {c: Logic} {b: Command}: [Hoare| ...] := sorry
+
+    theorem HoareLogic.complete {P Q: Assertion} {c: Command} (h: [Hoare| ⦃ ‹P› ⦄ ‹c› ⦃ ‹Q› ⦄]): HoareLogic P c Q := sorry
+  end Term
 
   /-
   ## Postscript: Decidability
