SoftwareFoundations/ProgrammingLanguageFoundations/SmallStep.lean
@@ -1,0 +1,515 @@
+/-
+# Small-Step Operational Semantics
+-/
+
+namespace SoftwareFoundations.ProgrammingLanguageFoundations.SmallStep
+  /-
+  ## A Toy Language
+  -/
+
+  inductive Term: Type where
+    | const (n: Nat): Term
+    | plus (t₁ t₂: Term): Term
+  deriving Repr
+
+  declare_syntax_cat toy
+
+  syntax num : toy
+  syntax:max "‹" term "›" : toy
+  syntax:max "‹‹" term "››" : toy
+  syntax:60 toy:60 "+" toy:61 : toy
+  syntax "(" toy ")" : toy
+
+  syntax "[Toy|" toy "]" : term
+
+  macro_rules
+    | `([Toy| $n:num])         => `(Term.const $n)
+    | `([Toy| ‹ $n:term ›])    => `(Term.const $(Lean.quote n))
+    | `([Toy| ‹‹ $t:term ›› ]) => `($(Lean.quote t))
+    | `([Toy| $t₁ + $t₂])      => `(Term.plus [Toy| $t₁] [Toy| $t₂])
+    | `([Toy| ( $t )])         => `([Toy| $t])
+
+  def Term.eval: Term → Nat
+    | .const n => n
+    | .plus t₁ t₂ => t₁.eval + t₂.eval
+
+  example: [Toy| (1 + 2) + (3 + 4)].eval = 10 := rfl
+
+  inductive Eval: Term → Nat → Prop where
+    | const {n: Nat}: Eval [Toy| ‹n›] n
+    | plus {t₁ t₂: Term} {n₁ n₂: Nat}: Eval t₁ n₁ → Eval t₂ n₂ → Eval [Toy| ‹‹t₁››  + ‹‹t₂››] (n₁ + n₂)
+
+  notation t "⇓" n => Eval t n
+
+  namespace SimpleArith
+    inductive Eval₁: Term → Term → Prop where
+      | constConst {n₁ n₂: Nat}: Eval₁ [Toy| ‹n₁› + ‹n₂›] [Toy| ‹n₁ + n₂›]
+      | plusL {t₁ t₂ t₃: Term} (h: Eval₁ t₁ t₂): Eval₁ [Toy| ‹‹t₁›› + ‹‹t₃››] [Toy| ‹‹t₂›› + ‹‹t₃››]
+      | plusR {n: Nat} {t₁ t₂: Term} (h: Eval₁ t₁ t₂): Eval₁ [Toy| ‹n› + ‹‹t₁››] [Toy| ‹n› + ‹‹t₂››]
+
+    scoped notation t₁ "⟶" t₂ => Eval₁ t₁ t₂
+
+    namespace Term
+      example: [Toy| (1 + 3) + (2 + 4)] ⟶ [Toy| 4 + (2 + 4)] :=
+        .plusL .constConst
+
+      example: [Toy| 0 + (2 + (1 + 3))] ⟶ [Toy| 0 + (2 + 4)] :=
+        .plusR (.plusR .constConst)
+    end Term
+
+    namespace Tactic
+      example: [Toy| (1 + 3) + (2 + 4)] ⟶ [Toy| 4 + (2 + 4)] := by
+        apply Eval₁.plusL
+        · apply Eval₁.constConst
+
+      example: [Toy| 0 + (2 + (1 + 3))] ⟶ [Toy| 0 + (2 + 4)] := by
+        apply Eval₁.plusR
+        · apply Eval₁.plusR
+          · apply Eval₁.constConst
+    end Tactic
+
+    namespace Blended
+      example: [Toy| (1 + 3) + (2 + 4)] ⟶ [Toy| 4 + (2 + 4)] :=
+        .plusL .constConst
+
+      example: [Toy| 0 + (2 + (1 + 3))] ⟶ [Toy| 0 + (2 + 4)] :=
+        .plusR (.plusR .constConst)
+    end Blended
+  end SimpleArith
+
+  /-
+  ## Relations
+  -/
+
+  def Relation (α: Type): Type := α → α → Prop
+
+  def Relation.deterministic (R: Relation α): Prop := ∀ {x y₁ y₂: α}, (h₁: R x y₁) → (h₂: R x y₂) → y₁ = y₂
+
+  namespace SimpleArith2
+    open SimpleArith
+
+    namespace Term
+      theorem Eval₁.deterministic: Relation.deterministic Eval₁
+        | _, _, _, .constConst, .constConst => rfl
+        | _, _, _, .plusL h₁, .plusL h₂ =>
+          have ih := deterministic h₁ h₂
+          calc Term.plus _ _
+            _ = Term.plus _ _ := congrFun (congrArg Term.plus ih) _
+        | _, _, _, .plusR h₁, .plusR h₂ =>
+          have ih := deterministic h₁ h₂
+          calc Term.plus (.const _) _
+            _ = Term.plus (.const _) _ := congrArg (Term.plus (.const _)) ih
+    end Term
+
+    namespace Tactic
+      theorem Eval₁.deterministic: Relation.deterministic Eval₁ := by
+        intro _ _ _
+        intro h₁ h₂
+        cases h₁ <;> cases h₂ <;> try (first | rfl
+                                             | contradiction)
+        case plusL.plusL _ _ _ h₁ _ h₂ => rw [deterministic h₁ h₂]
+        case plusR.plusR _ _ _ h₁ _ h₂ => rw [deterministic h₁ h₂]
+    end Tactic
+
+    namespace Blended
+      theorem Eval₁.deterministic: Relation.deterministic Eval₁
+        | _, _, _, .constConst, .constConst => by rfl
+        | _, _, _, .plusL h₁, .plusL h₂
+        | _, _, _, .plusR h₁, .plusR h₂ => by rw [deterministic h₁ h₂]
+    end Blended
+  end SimpleArith2
+
+  /-
+  ### Values
+  -/
+
+  inductive Value: Term → Prop where
+    | const (n: Nat): Value [Toy| ‹n›]
+
+  inductive Eval₁: Term → Term → Prop where
+    | constConst {n₁ n₂: Nat}: Eval₁ [Toy| ‹n₁› + ‹n₂›] [Toy| ‹n₁ + n₂›]
+    | plusL {t₁ t₂ t₃: Term} (h: Eval₁ t₁ t₂): Eval₁ [Toy| ‹‹t₁›› + ‹‹t₃››] [Toy| ‹‹t₂›› + ‹‹t₃››]
+    | plusR {v₁ t₁ t₂: Term} (h₁: Value v₁) (h₂: Eval₁ t₁ t₂): Eval₁ [Toy| ‹‹v₁›› + ‹‹t₁››] [Toy| ‹‹v₁›› + ‹‹t₂››]
+
+  notation t₁ "⟶" t₂ => Eval₁ t₁ t₂
+
+  namespace Term
+    theorem Eval₁.deterministic: Relation.deterministic Eval₁
+      | _, _, _, .constConst, .constConst => rfl
+      | _, _, _, .plusL h₁, .plusL h₂ =>
+        have ih := deterministic h₁ h₂
+        calc Term.plus _ _
+          _ = Term.plus _ _ := congrFun (congrArg Term.plus ih) _
+      | _, _, _, .plusR hv h₁, .plusL h₂ =>
+        sorry
+      | _, _, _, .plusR hv₁ h₁, .plusR hv₂ h₂ =>
+        have ih := deterministic h₁ h₂
+        -- calc Term.plus (.const _) _
+        --   _ = Term.plus (.const _) _ := congrArg (Term.plus (.const _)) ih
+        sorry
+  end Term
+
+  namespace Tactic
+    theorem Eval₁.deterministic: Relation.deterministic Eval₁ := by
+      intro _ _ _
+      intro h₁ h₂
+      cases h₁ <;> cases h₂ <;> try (first | rfl
+                                           | contradiction)
+      case plusL.plusL _ _ _ h₁ _ h₂       => rw [deterministic h₁ h₂]
+      case plusR.plusR _ _ hv₁ h₁ _ hv₂ h₂ => rw [deterministic h₁ h₂]
+      case plusL.plusR _ _ _ h₁ _ hv h₂    => sorry
+      case plusR.plusL _ _ _ hv h₁ _ h₂    => sorry
+  end Tactic
+
+  namespace Blended
+    theorem Eval₁.deterministic: Relation.deterministic Eval₁
+      | _, _, _, .constConst, .constConst => by rfl
+      | _, _, _, .plusL h₁, .plusL h₂ => by rw [deterministic h₁ h₂]
+      | _, _, _, .plusR hv₁ h₁, .plusR hv₂ h₂ => by rw [deterministic h₁ h₂]
+      | _, _, _, .plusR hv h₁, .plusL h₂ => sorry
+  end Blended
+
+  /-
+  ### Strong Progress and Normal Forms
+  -/
+
+  namespace Term
+    theorem Eval₁.strong_progress: ∀ t₁: Term, Value t₁ ∨ ∃ t₂: Term, t₁ ⟶ t₂
+      | .const n => .inl (.const n)
+      | .plus t₁ t₂ =>
+        match strong_progress t₁, strong_progress t₂ with
+          | .inl (.const n₁), .inl (.const n₂) => .inr ⟨.const (n₁ + n₂), .constConst⟩
+          | .inl (.const n₁), .inr ⟨t₃, hw⟩    => .inr ⟨.plus (.const n₁) t₃, .plusR (.const n₁) hw⟩
+          | .inr ⟨t₃, hw⟩, _                   => .inr ⟨.plus t₃ t₂, .plusL hw⟩
+  end Term
+
+  namespace Tactic
+    theorem Eval₁.strong_progress: ∀ t₁: Term, Value t₁ ∨ ∃ t₂: Term, t₁ ⟶ t₂ := by
+      intro t₁
+      induction t₁ with
+        | const n =>
+          apply Or.inl
+          · apply Value.const
+        | plus t₁ t₂ ih₁ ih₂ =>
+          cases ih₁ with
+            | inr ex =>
+              apply Or.inr
+              · apply Exists.intro
+                · apply Eval₁.plusL
+                  · sorry
+                  · sorry
+            | inl hv₁ =>
+              cases ih₂ with
+                | inr ex =>
+                  apply Or.inr
+                  · apply Exists.intro
+                    · apply Eval₁.plusR
+                      · exact hv₁
+                      · sorry
+                      · sorry
+                | inl hv₂ =>
+                  cases t₁ with
+                    | plus _ _ => contradiction
+                    | const n₁ =>
+                      cases t₂ with
+                        | plus _ _ => contradiction
+                        | const n₂ =>
+                          apply Or.inr
+                          · apply Exists.intro
+                            · apply Eval₁.constConst
+  end Tactic
+
+  namespace Blended
+    theorem Eval₁.strong_progress: ∀ t₁: Term, Value t₁ ∨ ∃ t₂: Term, t₁ ⟶ t₂
+      | .const n => .inl (.const n)
+      | .plus t₁ t₂ =>
+        match strong_progress t₁, strong_progress t₂ with
+          | .inl (.const n₁), .inl (.const n₂) => .inr ⟨.const (n₁ + n₂), .constConst⟩
+          | .inl (.const n₁), .inr ⟨t₃, hw⟩    => .inr ⟨.plus (.const n₁) t₃, .plusR (.const n₁) hw⟩
+          | .inr ⟨t₃, hw⟩, _                   => .inr ⟨.plus t₃ t₂, .plusL hw⟩
+  end Blended
+
+  def Relation.normal (R: Relation α) (t₁: α): Prop := ¬ ∃ t₂: α, R t₁ t₂
+
+  namespace Term
+    theorem Value.normal {v: Term}: Value v → Relation.normal Eval₁ v
+      | .const n₁, ⟨w, hw⟩ =>
+        -- by contradiction
+        sorry
+
+    theorem Relation.normal.value {t: Term}: Relation.normal Eval₁ t → Value t
+      | hn =>
+        match Eval₁.strong_progress t with
+          | .inl hv => hv
+          | .inr hex => absurd hex hn
+
+    theorem normal_value {t: Term}: Relation.normal Eval₁ t ↔ Value t :=
+      ⟨Relation.normal.value, Value.normal⟩
+  end Term
+
+  namespace Tactic
+    theorem Value.normal {v: Term}: Value v → Relation.normal Eval₁ v := by
+      intro hv
+      intro
+      | .intro w hw =>
+        cases hv with
+          | const n => contradiction
+
+    theorem Relation.normal.value {t: Term}: Relation.normal Eval₁ t → Value t := by
+      intro hn
+      have h: Value t ∨ ∃ t₂: Term, t ⟶ t₂ := by
+        apply Eval₁.strong_progress
+      cases h with
+        | inl _ => assumption
+        | inr _ => contradiction
+
+    theorem normal_value {t: Term}: Relation.normal Eval₁ t ↔ Value t := by
+      apply Iff.intro
+      · exact Relation.normal.value
+      · exact Value.normal
+  end Tactic
+
+  namespace Blended
+    theorem Value.normal {v: Term}: Value v → Relation.normal Eval₁ v
+      | .const n₁, ⟨.const n₂, hw⟩ => by contradiction
+
+    theorem Relation.normal.value {t: Term}: Relation.normal Eval₁ t → Value t
+      | hn =>
+        match Eval₁.strong_progress t with
+          | .inl hv => hv
+          | .inr hex => absurd hex hn
+
+    theorem normal_value {t: Term}: Relation.normal Eval₁ t ↔ Value t :=
+      ⟨Relation.normal.value, Value.normal⟩
+  end Blended
+
+  namespace Temp1
+    inductive Value: Term → Prop where
+      | const (n: Nat): Value [Toy| ‹n›]
+      | funny (t₁: Term) (n: Nat): Value [Toy| ‹‹t₁›› + ‹n›]
+
+    inductive Eval₁: Term → Term → Prop where
+      | constConst {n₁ n₂: Nat}: Eval₁ [Toy| ‹n₁› + ‹n₂›] [Toy| ‹n₁ + n₂›]
+      | plusL {t₁ t₂ t₃: Term} (h: Eval₁ t₁ t₂): Eval₁ [Toy| ‹‹t₁›› + ‹‹t₃››] [Toy| ‹‹t₂›› + ‹‹t₃››]
+      | plusR {v₁ t₁ t₂: Term} (h₁: Value v₁) (h₂: Eval₁ t₁ t₂): Eval₁ [Toy| ‹‹v₁›› + ‹‹t₁››] [Toy| ‹‹v₁›› + ‹‹t₂››]
+
+    notation t₁ "⟶" t₂ => Eval₁ t₁ t₂
+
+    -- def Relation.normal (R: Relation α) (t₁: α): Prop := ¬ ∃ t₂: α, R t₁ t₂
+
+    namespace Term
+      theorem value_not_normal_form: ∃ v: Term, Value v ∧ ¬Relation.normal Eval₁ v :=
+        have hwv := .funny [Toy| 1 + 2] 3
+        have hwnn
+          | hn => hn ⟨[Toy| 3 + 3], .plusL .constConst⟩
+        ⟨[Toy| (1 + 2) + 3], ⟨hwv, hwnn⟩⟩
+    end Term
+
+    namespace Tactic
+      theorem value_not_normal_form: ∃ v: Term, Value v ∧ ¬Relation.normal Eval₁ v := by
+        apply Exists.intro
+        · apply And.intro
+          · apply Value.funny
+            · exact [Toy| 1 + 2]
+            · exact 3
+          . unfold Relation.normal
+            intro hn
+            apply hn
+            · apply Exists.intro
+              · apply Eval₁.plusL
+                · apply Eval₁.constConst
+    end Tactic
+
+    namespace Blended
+      theorem value_not_normal_form: ∃ v: Term, Value v ∧ ¬Relation.normal Eval₁ v :=
+        have hwv := .funny [Toy| 1 + 2] 3
+        have hwnn
+          | hn => hn ⟨[Toy| 3 + 3], .plusL .constConst⟩
+        ⟨[Toy| (1 + 2) + 3], ⟨hwv, hwnn⟩⟩
+    end Blended
+  end Temp1
+
+  namespace Temp2
+    inductive Value: Term → Prop where
+      | const (n: Nat): Value [Toy| ‹n›]
+
+    inductive Eval₁: Term → Term → Prop where
+      | funny {n: Nat}: Eval₁ [Toy| ‹n›] [Toy| ‹n› + 0]
+      | constConst {n₁ n₂: Nat}: Eval₁ [Toy| ‹n₁› + ‹n₂›] [Toy| ‹n₁ + n₂›]
+      | plusL {t₁ t₂ t₃: Term} (h: Eval₁ t₁ t₂): Eval₁ [Toy| ‹‹t₁›› + ‹‹t₃››] [Toy| ‹‹t₂›› + ‹‹t₃››]
+      | plusR {v₁ t₁ t₂: Term} (h₁: Value v₁) (h₂: Eval₁ t₁ t₂): Eval₁ [Toy| ‹‹v₁›› + ‹‹t₁››] [Toy| ‹‹v₁›› + ‹‹t₂››]
+
+    notation t₁ "⟶" t₂ => Eval₁ t₁ t₂
+
+    -- def Relation.normal (R: Relation α) (t₁: α): Prop := ¬ ∃ t₂: α, R t₁ t₂
+
+    namespace Term
+      theorem value_not_normal_form: ∃ v: Term, Value v ∧ ¬Relation.normal Eval₁ v :=
+        have hv := .const 1
+        have hnn
+          | hn => hn ⟨[Toy| 1 + 0], .funny⟩
+        ⟨[Toy| 1], ⟨hv, hnn⟩⟩
+    end Term
+
+    namespace Tactic
+      theorem value_not_normal_form: ∃ v: Term, Value v ∧ ¬Relation.normal Eval₁ v := by
+        apply Exists.intro
+        · apply And.intro
+          · apply Value.const
+            · exact 1
+          . unfold Relation.normal
+            intro hn
+            apply hn
+            · apply Exists.intro
+              · apply Eval₁.funny
+    end Tactic
+
+    namespace Blended
+      theorem value_not_normal_form: ∃ v: Term, Value v ∧ ¬Relation.normal Eval₁ v :=
+        have hv := .const 1
+        have hnn
+          | hn => hn ⟨[Toy| 1 + 0], .funny⟩
+        ⟨[Toy| 1], ⟨hv, hnn⟩⟩
+    end Blended
+  end Temp2
+
+  namespace Temp3
+    inductive Value: Term → Prop where
+      | const (n: Nat): Value [Toy| ‹n›]
+
+    inductive Eval₁: Term → Term → Prop where
+      | constConst {n₁ n₂: Nat}: Eval₁ [Toy| ‹n₁› + ‹n₂›] [Toy| ‹n₁ + n₂›]
+      | plusL {t₁ t₂ t₃: Term} (h: Eval₁ t₁ t₂): Eval₁ [Toy| ‹‹t₁›› + ‹‹t₃››] [Toy| ‹‹t₂›› + ‹‹t₃››]
+
+    notation t₁ "⟶" t₂ => Eval₁ t₁ t₂
+
+    -- def Relation.normal (R: Relation α) (t₁: α): Prop := ¬ ∃ t₂: α, R t₁ t₂
+
+    namespace Term
+      theorem value_not_normal_form: ∃ v: Term, ¬Value v ∧ Relation.normal Eval₁ v :=
+        have hnv
+          | hv => sorry
+        have hn
+          | ⟨w, hnw⟩ => sorry
+        ⟨[Toy| 1 + (2 + 3)], ⟨hnv, hn⟩⟩
+    end Term
+
+    namespace Tactic
+      theorem value_not_normal_form: ∃ v: Term, ¬Value v ∧ Relation.normal Eval₁ v := by
+        apply Exists.intro
+        · apply And.intro
+          · intro hnv
+            sorry
+          · unfold Relation.normal
+            intro hn
+            sorry
+        sorry
+    end Tactic
+
+    namespace Blended
+      theorem value_not_normal_form: ∃ v: Term, ¬Value v ∧ Relation.normal Eval₁ v := sorry
+    end Blended
+  end Temp3
+
+  namespace Temp4
+    inductive Term: Type where
+      | true: Term
+      | false: Term
+      | test: Term → Term → Term → Term
+
+    declare_syntax_cat tf
+
+    syntax "tru" : tf
+    syntax "fls" : tf
+    syntax:max "‹" term "›" : tf
+    syntax "test" "(" tf ")" "{" tf "}" "else" "{" tf "}" : tf
+    syntax "(" tf ")" : tf
+
+    syntax "[TF|" tf "]" : term
+
+    macro_rules
+      | `([TF| tru])                            => `(Term.true)
+      | `([TF| fls])                            => `(Term.false)
+      | `([TF| ‹ true ›])                       => `(Term.const true)
+      | `([TF| ‹ false ›])                      => `(Term.const false)
+      | `([TF| ‹ $t:term ›])                    => `($(Lean.quote t))
+      | `([TF| test ( $c ) { $t } else { $f }]) => `(Term.test [TF| $c] [TF| $t] [TF| $f])
+      | `([TF| ( $t )])                         => `([TF| $t])
+
+    inductive Value: Term → Prop where
+      | true: Value .true
+      | false: Value .false
+
+    inductive Eval₁: Term → Term → Prop where
+      | testTrue {t f: Term}: Eval₁ [TF| test (tru) { ‹t› } else { ‹f› }] t
+      | testFalse {t f: Term}: Eval₁ [TF| test (fls) { ‹t› } else { ‹f› }] f
+      | test {c₁ c₂ t f: Term} (h: Eval₁ c₁ c₂): Eval₁ [TF| test (‹c₁›) { ‹t› } else { ‹f› }] [TF| test (‹c₂›) { ‹t› } else { ‹f› }]
+
+    notation t₁ "⟶" t₂ => Eval₁ t₁ t₂
+
+    -- TODO: Which propositions are provable
+
+    namespace Term
+      theorem Eval₁.strong_progress: ∀ t₁: Term, Value t₁ ∨ ∃ t₂: Term, Eval₁ t₁ t₂
+        | .true => .inl .true
+        | .false => .inl .false
+        | .test c t f =>
+          match strong_progress c, strong_progress t, strong_progress f with
+            | .inl .true, _, _ => .inr ⟨[TF| ‹t›], .testTrue⟩
+            | .inl .false, _, _ => .inr ⟨[TF| ‹f›], .testFalse⟩
+            | .inr ⟨w, hw⟩, _, _ => .inr ⟨[TF| test (‹w›) { ‹t›} else { ‹f› }], .test hw⟩
+
+      theorem Eval₁.deterministic: Relation.deterministic Eval₁
+        | _, _, _, .testTrue, .testTrue
+        | _, _, _, .testFalse, .testFalse => rfl
+        | _, _, _, .test h₁, .test h₂ =>
+          have ih := deterministic h₁ h₂
+          calc Term.test _ _ _
+            _ = Term.test _ _ _ := by rw [ih] -- TODO: Remove Tactic Block
+    end Term
+
+    namespace Tactic
+      theorem Eval₁.strong_progress: ∀ t₁: Term, Value t₁ ∨ ∃ t₂: Term, Eval₁ t₁ t₂ := sorry
+
+      theorem Eval₁.deterministic: Relation.deterministic Eval₁ := by
+        intro _ _ _ h₁ h₂
+        cases h₁ <;> cases h₂ <;> try (first | rfl
+                                             | contradiction)
+        case test.test _ _ _ _ h₁ _ h₂ => rw [deterministic h₁ h₂]
+    end Tactic
+
+    namespace Blended
+      theorem Eval₁.strong_progress: ∀ t₁: Term, Value t₁ ∨ ∃ t₂: Term, Eval₁ t₁ t₂
+        | .true => .inl .true
+        | .false => .inl .false
+        | .test c t f =>
+          match strong_progress c, strong_progress t, strong_progress f with
+            | .inl .true, _, _ => .inr ⟨[TF| ‹t›], .testTrue⟩
+            | .inl .false, _, _ => .inr ⟨[TF| ‹f›], .testFalse⟩
+            | .inr ⟨w, hw⟩, _, _ => .inr ⟨[TF| test (‹w›) { ‹t›} else { ‹f› }], .test hw⟩
+
+      theorem Eval₁.deterministic: Relation.deterministic Eval₁
+        | _, _, _, .testTrue, .testTrue => rfl
+        | _, _, _, .testFalse, .testFalse => rfl
+        | _, _, _, .test h₁, .test h₂ => by rw [deterministic h₁ h₂]
+    end Blended
+
+    namespace Temp5
+      inductive Eval₁: Term → Term → Prop where
+        | testTrue {t f: Term}: Eval₁ [TF| test (tru) { ‹t› } else { ‹f› }] t
+        | testFalse {t f: Term}: Eval₁ [TF| test (fls) { ‹t› } else { ‹f› }] f
+        | test {c₁ c₂ t f: Term} (h: Eval₁ c₁ c₂): Eval₁ [TF| test (‹c₁›) { ‹t› } else { ‹f› }] [TF| test (‹c₂›) { ‹t› } else { ‹f› }]
+        | shortCircuit {c t₁ t₂ f₁ f₂} (h₁: Eval t₁ t₂) (h₂: Eval f₁ f₂) (h₃: t₂ = f₂): Eval₁ [TF| test (‹c›) { ‹t₁› } else { ‹f₁› }] t₁
+
+      notation t₁ "⟶" t₂ => Eval₁ t₁ t₂
+
+      -- TODO
+    end Temp5
+  end Temp4
+
+  /-
+  ## Multi-Step Reduction
+  -/
+
+
+end SoftwareFoundations.ProgrammingLanguageFoundations.SmallStep
